setting up the notion of depth for bfs

examples/data_structures/graph/Graph.Traversal.fst
@@ -1,1 +1,40 @@
 module Graph.Traversal
+
+open Graph.Base
+open Seq.Complements
+module SEM = FStar.StrongExcludedMiddle
+
+(* `depth g root x d` holds iff the depth of x in the graph rooted in root is d *)
+(* where None = \infty *)
+let depth (#n:nat) (g:graph0 n) (root x:_in g) (d:option nat) =
+  match d with
+  | None -> (forall (p:path g). from p == root ==> to p =!= x)
+  | Some k ->
+    (exists (p:path g). from p == root /\ to p == x /\ length p == k) /\
+    (forall (p:path g). from p == root /\ to p == x ==> length p >= k)
+
+let lemma_path_max_length (#n:nat) (g:graph0 n) (root x : _in g)
+  : Lemma (requires (forall (p:path g). from p == root /\ to p == x ==> length p >= n+1))
+          (ensures (forall (p:path g). from p == root ==> to p =!= x))
+(* TODO : prove me ! *)
+= admit ()
+
+let rec depth_fun_aux (#n:nat) (g:graph0 n) (root x:_in g) (k:nat)
+  : Ghost (option nat)
+    (requires (forall (p:path g). from p == root /\ to p == x ==> length p >= k))
+    (ensures (depth g root x))
+    (decreases (n+1-k))
+= if k > n then (lemma_path_max_length g root x ; None)
+  else if SEM.strong_excluded_middle (exists (p:path g). from p == root /\ to p == x /\ length p == k)
+  then Some k
+  else depth_fun_aux g root x (k+1)
+
+let depth_fun (#n:nat) (g:graph0 n) (root x:_in g) : GTot (d:option nat{depth g root x d}) =
+  depth_fun_aux g root x 0
+
+
+type traversal (#n:nat) (g:graph0 n) (root:_in g) : nodeset n -> Type0 =
+  fun s ->
+    Cons? s /\
+    Cons?.hd s == root (* /\ *)
+    (* missing condition ... *)
